\documentclass[en,skiptitle,skiptoc]{../../../eplerrata}

\DeclareExpandableDocumentCommand{\erratumcorrected}{mmmmmm}{\erratum[It is how it was corrected in \cite[p.~#1, l.~$#2$]{nesterov2004introductory}.]{#3}{#4}{#5}{#6}}

\title{Nonlinear programming: INMA2460}
\author{Benoît Legat}

\hypertitle{Nonlinear programming}{8}{INMA}{2460}
{Benoît Legat}
{Yurii Nesterov}

\maketitle

\section{Introductory Lectures on Convex Programming~\cite{nesterov1998introductory}}

\begin{errata}
  \erratum{5}{-4}{May be}{Maybe}
  \erratumcorrected{xvi}{-13}{6}{9}{been never}{never been}
  \erratum{7}{16}{cam}{can}
  \erratum{14}{13}{$\la x, x \ra$}{$\sqrt{\la x, x \ra}$ ou $\la x, x \ra^{\frac{1}{2}}$}
  \erratum{15}{-5}{$\lfloor L \frac{\sqrt{n}}{2\epsilon} \rfloor \lfloor$}{$\lfloor L \frac{\sqrt{n}}{2\epsilon} \rfloor$}
  \erratum{16}{-12}{$]\frac{L}{2\epsilon}[$}{$\lfloor \frac{L}{2\epsilon} \rfloor$}
  \erratumcorrected{12}{-1}{18}{13}{let we}{if we}
  \erratumcorrected{13}{-12}{18}{-8}{may be}{maybe}
  \erratum{21}{-12}{$\lim_{y_k \to x_k}$}{$\lim_{y_k \to \bar{x}}$}
  \erratum{22}{1}{$f'(\bar{x}$}{$f'(\bar{x})$}
  \erratumcorrected{18}{5}{22}{13}{$\la f'(x^*), s \ra = 0$}{$\la f'(x^*), s \ra \geq 0$}
  \erratum[We use Lemma~1.2.3 \cite[p.~39 l.~4]{nesterov1998introductory}]{38}{-16}{$f \in C_L^{2,2}$}{$f \in C_L^{1,1}$}
  \erratum{43}{-6}{$\fpart{\phi(\lambda_*)}{\lambda^{i}}$}{$2\la f'(x_k), f'(x_i) \ra$}
  \erratum[$f$ is not defined here, the objective is $f_0$.]{47}{-8}{$\lim_{k \to \infty} f(x_k)$}{$\lim_{k \to \infty} f_0(x_k)$}
  \erratum{47}{-1}
  {we have $\Phi(x_*)=0$. Therefore $x_* \in Q$ and $\Psi^* = f_0(x_*) + \Phi(x_*) = f_0(x_*) \geq f^*$.}
  {See the errata of~\cite{nesterov2004introductory}.}
  \erratum{69}{-2}{$\phi_{k+1}^* = (1-\alpha_k)\phi_k$}{$\phi_{k+1}^* = (1-\alpha_k)\phi_k^*$}
  \erratum{71}{6}{$x_{k+1}=y_k-h_kf'(x_k)$}{$x_{k+1}=y_k-h_kf'(y_k)$}
  \erratum{81}{10}{$x_Q=x_Q(\gamma,\bar{x}),g_Q=g_Q(\gamma,\bar{x})$}{$x_Q=x_Q(\bar{x};\gamma),g_Q=g_Q(\bar{x};\gamma)$}
  \erratumcorrected{89}{5}{83}{1}{$\{\phi)k(x)\}$}{$\{\phi_k(x)\}$}
  \erratumcorrected{118}{-8}{109}{-2}{$\phi(\mathcal{A}(x)$}{$\phi(\mathcal{A}(x))$}
  \erratumcorrected{121}{-1}{112}{-8}{Lipshitz}{Lipschitz}
  \erratumcorrected{127}{6}{117}{7}{cinvexity}{convexity}
  \erratum{119}{-11}{$\la g, x_0-x$}{$\la  g, x_0-x \ra$}
  \erratumcorrected{137}{-15}{126}{3}{staring}{starting}
  \erratumcorrected{140}{8}{128}{-16}{$\omega_f(v_f(\bar{x};x))$}{$\omega_f(\bar{x}; v_f(\bar{x};x))$}
  \erratumcorrected{140}{17}{128}{-7}{$\la g(x), y - x \ra$}{$\la g(x), y - \bar{x} \ra$}
  \erratumcorrected{137}{8}{129}{9}{$\omega_f(v_k^*)$}{$\omega_f(x^*; v_k^*)$}
  \erratum{130}{-2}{$f_k^*$}{$f_N^*$}
  \erratumcorrected{143}{-6}{131}{8}{3.2.3)}{(3.2.3)}
  \erratum{131}{-17}{$i=1 \ldots m$}{$j=1, \ldots, m$}
  \erratumcorrected{146}{4}{133}{13}{iur}{our}
  \erratum{133}{-6}{abou}{about}
  \erratumcorrected{146}{-13}{133}{-5}{repotrts}{reports}
  \erratumcorrected{146}{-4}{134}{3}{$x \in Q$}{$, x \in Q$}
  \erratumcorrected{148}{5}{135}{-7}{inceased}{increased}
  \erratum{136}{12}{THe}{The}
  \erratumcorrected{148}{-3}{136}{-9}{thatthe}{thatthe}
  \erratumcorrected{150}{11}{138}{5}{Insted}{Instead}
  \erratumcorrected{151}{14}{139}{4}{immedeately}{immediately}
  \erratumcorrected{152}{-6}{140}{9}{certer}{center}
  \erratumcorrected{154}{-1}{142}{5}{$H_k^{-1}(x-x_k),x-x_k$}{$H_k^{-1}(x-y_k),x-y_k$}
  \erratum{142}{11}{$B_0(x_0,R)$}{$B_2(x_0,R)$}
  \erratumcorrected{155}{-8}{143}{1}{feasble}{feasible}
  \erratumcorrected{156}{2}{143}{9}{dependedce}{dependence}
  \erratumcorrected{156}{17}{143}{-9}{volumetrictic}{volumetric}
  %\erratum[Or say that $\|u\| = 1$]{160}{12}{$f'''(x)[u] = \lim_{\alpha \to 0} \frac{1}{\alpha}[f''(x+\alpha u) - f''(x)]$}{$f'''(x)[u] = \lim_{\alpha \to 0} \frac{1}{\alpha\|u\|}[f''(x+\alpha u) - f''(x)]$}
  \erratum{161}{2}{$\|u\|_{f''(x)}^{3/2}$}{$\|u\|_{f''(x)}^{3}$}
  \erratum{161}{12}{we put its proof in Appendix}{we won't prove it}
  \erratum{162}{13}{Thus, ...}{The last inequality can be proved by derivative or by the Bernoulli's inequality, using the fact that since $D^2f(x)[u,u] \geq 0$, $\alpha \geq -1$. Thus, ...}
  \erratum{164}{13}{$\psi'(\alpha) + \xi'(\alpha)$}{$\psi'(\alpha) + \xi(\alpha)$}
  \erratum[See the erratum for \cite[p.~143, l.~$-8$]{nesterov2004introductory}.]{131}{6}{$\frac{R^2+r\ln(k+1)}{2r\sqrt{k+1}}$}{$\frac{R^2+r^2\ln(k+1)}{4r\sqrt{k+1}}$}
  \erratum{177}{4--6}{$\la F'(x) u, u \ra$}{$\la F'(x), u \ra$}
  \erratum{181}{10}{$\|t_+c+F'(x_+)\|_x^*$}{$\|t_+c+F'(x_+)\|_{x_+}^*$}
  \erratum{184}{1}{$r = \|u\|_x = [\phi''(0)]^{-1/2}$}{$r = \|u\|_x = [\psi''(0)]^{-1/2}$}
  \erratum{184}{5}{$\frac{1}{6}\psi'''(0) = \lim_{\alpha \downarrow 0} [$}{$\frac{1}{6}\psi'''(0) = \lim_{\alpha \downarrow 0} \frac{1}{\alpha^3}[$}
  \erratum{184}{8}{$D^3f(x)[u,u,u] = -\psi''(0) \leq \psi'''(0) \leq 2[\psi''(0)]^{3/2}$}{$D^3f(x)[u,u,u] = -\psi'''(0) \leq 2[\psi''(0)]^{3/2}$}
\end{errata}

\section{Introductory Lectures on Convex Programming~\cite{nesterov2004introductory}}

\begin{errata}
  \erratum{9}{-1}{constrict}{construct}
  \erratum{17}{-10}{$f'(\bar{x}$}{$f'(\bar{x})$}
  \erratum{35}{-13}{$f''(x_k) \geq f''(x^*) - Mr_kI_n \geq (l-Mr_k)I_n$}{$f''(x_k) \succeq f''(x^*) - Mr_kI_n \succeq (l-Mr_k)I_n$}
  \erratum[We use Lemma~1.2.3 \cite[p.~38 l.~1]{nesterov2004introductory}]{38}{-16}{$f \in C_L^{2,2}$}{$f \in C_L^{1,1}$}
  \erratum{43}{8}{$\fpart{\phi(\lambda_*)}{\lambda^{i}} = \la f'(x_k), f'(x_i) \ra$}{$\fpart{\phi(\lambda_*)}{\lambda^{i}} = 2\la f'(x_k), f'(x_i) \ra$}
  \erratum[$f$ is not defined here, the objective is $f_0$.]{48}{9}{$\lim_{k \to \infty} f(x_k)$}{$\lim_{k \to \infty} f_0(x_k)$}
  \erratum[$f^*$ was used in \cite{nesterov1998introductory} and replaced by $f(x^*)$. This one was forgotten.]{48}{12}{$\Psi^* \leq f^*$}{$\Psi^* \leq f(x^*)$}
  \erratum[$\Psi^* = f_0(x_*) + \Phi(x_*) = f_0(x_*)$ is incorrect, which $t$ to use ? The limit ?
  The $\Phi(x_*) \lim t_k = 0 \cdot \infty$ so we cannot say much. Also the fact that $\lim t_k \to \infty$ is not the reason that $f_0(x_*) \leq f_0(x^*)$.]{48}{-13}
  {we have $\Phi(x_*)=0$ and $f_0(x_*) \leq f_0(x^*)$. Thus $x_* \in Q$ and $\Psi^* = f_0(x_*) + \Phi(x_*) = f_0(x_*) \geq f_0(x^*)$.}
  {we have $\Phi(x_*)=0$. Thus $x_* \in Q$ and $f_0(x_*) \geq f_0(x^*)$.
  Since $f_0(x_*) \leq \Psi^* \leq f_0(x^*)$, we can conclude that $f_0(x_*) = f_0(x^*)$.}
  \erratum{73}{-2}{$\phi_{k+1}^* = (1-\alpha_k)\phi_k$}{$\phi_{k+1}^* = (1-\alpha_k)\phi_k^*$}
  \erratum{75}{-11}{$x_{k+1}=y_k-h_kf'(x_k)$}{$x_{k+1}=y_k-h_kf'(y_k)$}
  \erratum{129}{-3}{$\la g, x_0-x$}{$\la  g, x_0-x \ra$}
  \erratum{143}{12}{$f_k^*$}{$f_N^*$}
  \erratum[we can upper bound the sum $\sum_{i=0}^{k} \frac{1}{i+1}$ by $1+\int_0^{k} \frac{1}{i+1} = 1+\ln(k+1)$ and
  lower bound the sum $\sum_{i=0}^{k} \frac{1}{\sqrt{i+1}}$ by $\int_0^{k+1} \frac{1}{\sqrt{i+1}} = 2(\sqrt{k+2}-1)$. We don't care about the difference between $k+1$ and $k+2$.]{143}{-8}{$\frac{R^2+r\ln(k+1)}{2r\sqrt{k+1}}$}{$\frac{R^2+r^2\ln(k+1)}{4r\sqrt{k+1}}$}
  \erratum{144}{4}{$i=1 \ldots m$}{$j=1, \ldots, m$}
  \erratum{155}{8}{$B_0(x_0,R)$}{$B_2(x_0,R)$}
  %%\erratum[Or say that $\|u\| = 1$]{175}{9}{$f'''(x)[u] = \lim_{\alpha \to 0} \frac{1}{\alpha}[f''(x+\alpha u) - f''(x)]$}{$f'''(x)[u] = \lim_{\alpha \to 0} \frac{1}{\alpha\|u\|}[f''(x+\alpha u) - f''(x)]$}
  \erratum{176}{3}{$\|u\|_{f''(x)}^{3/2}$}{$\|u\|_{f''(x)}^{3}$}
  \erratum{177}{-5}{Thus, ...}{The last inequality can be proved by derivative or by the Bernoulli's inequality, using the fact that since $D^2f(x)[u,u] \geq 0$, $\alpha \geq -1$. Thus, ...}
  \erratum{184}{1}{$r = \|u\|_x = [\phi''(0)]^{-1/2}$}{$r = \|u\|_x = [\psi''(0)]^{-1/2}$}
  \erratum{184}{5}{$\frac{1}{6}\psi'''(0) = \lim_{\alpha \downarrow 0} [$}{$\frac{1}{6}\psi'''(0) = \lim_{\alpha \downarrow 0} \frac{1}{\alpha^3}[$}
  \erratum{184}{8}{$D^3f(x)[u,u,u] = -\psi''(0) \leq \psi'''(0) \leq 2[\psi''(0)]^{3/2}$}{$D^3f(x)[u,u,u] = -\psi'''(0) \leq 2[\psi''(0)]^{3/2}$}
  \erratum{187}{10--11}{}{$\la \phi'(y),z-y \ra \leq \|\phi'(y)\|_y^*  \|z-y\|_y$ but we would need a $-$ because after we use $-\omega(t) = \min -\xi t + \omega_*(\xi)$ of Lemma~4.1.4.}
  \erratum{196}{3--6}{$\la F'(x) u, u \ra$}{$\la F'(x), u \ra$}
  \erratum{201}{-13}{$\|t_+c+F'(x_+)\|_x^*$}{$\|t_+c+F'(x_+)\|_{x_+}^*$}
  \erratum{205}{2}{$x_0$}{$y_0$}
  \erratum{205}{9}{$t_{k+1}F'(y_0)-F'(y_k)$}{$-t_{k+1}F'(y_0)+F'(y_k)$}
  \erratum{205}{15}{$t_kF'(y_0)-F'(y_k)$}{$-t_kF'(y_0)+F'(y_k)$}
  \erratum{206}{5}{$\exp(...)$}{$\exp(...)t_0$}
  \erratum{206}{7}{$(t_kF'(x_0)+F'(y_k))-t_kF'(x_0)$}{$(-t_kF'(y_0)+F'(y_k))+t_kF'(y_0)$}
  \erratum{206}{10}{$F'(x_0)$}{$F'(y_0)$}
  \erratum{209}{10}{$z^*$}{$z_*$}
\end{errata}

\biblio

\end{document}
